common/Common.ConnectionStateQuery.fst
@@ -4,72 +4,80 @@ module Common.ConnectionStateQuery
 
 open Pulse.Lib.Pervasives
 
+module CPI = Common.ProtocolImplementation
 module TCP = Common.TCP
 
 noextract
 class connection_state_query
   (impl:Type0)
   (state:Type0)
+  (wire_message:Type0)
+  (local_event:Type0)
+  (local_output:Type0)
   (query:Type0)
-  (result:Type0)
+  (action:Type0)
+  (protocol:CPI.protocol_implementation
+    impl
+    state
+    wire_message
+    local_event
+    local_output)
   =
 {
-  csq_invariant:
-    impl ->
-    TCP.bytes ->
-    TCP.bytes ->
-    state ->
-    slprop;
-
   csq_frame:
     Type0;
 
   csq_frame_pre:
+    impl ->
     query ->
     csq_frame ->
     state ->
     slprop;
 
   csq_frame_post:
+    impl ->
     query ->
     csq_frame ->
     state ->
-    result ->
+    action ->
     slprop;
 
-  csq_sound:
+  csq_action_sound:
+    impl ->
     query ->
     state ->
-    result ->
+    action ->
     prop;
 
-  csq_run:
+  csq_next_action:
     i:impl ->
     q:query ->
     frame:csq_frame ->
     received:Ghost.erased TCP.bytes ->
     sent:Ghost.erased TCP.bytes ->
     st:Ghost.erased state ->
-      stt result
-        (csq_invariant
+      stt action
+        (protocol.CPI.pi_invariant
           i
           (Ghost.reveal received)
           (Ghost.reveal sent)
           (Ghost.reveal st) **
          csq_frame_pre
+          i
           q
           frame
           (Ghost.reveal st))
-        (fun result ->
-          csq_invariant
+        (fun action ->
+          protocol.CPI.pi_invariant
             i
             (Ghost.reveal received)
             (Ghost.reveal sent)
             (Ghost.reveal st) **
           csq_frame_post
+            i
             q
             frame
             (Ghost.reveal st)
-            result **
-          pure (csq_sound q (Ghost.reveal st) result));
+            action **
+          pure (csq_action_sound i q (Ghost.reveal st) action));
 }
